HumanProof/Meta/Abstraction.lean
@@ -1,0 +1,118 @@
+import Lean
+import Qq
+import Mathlib.Util.AtomM
+
+namespace Abstraction
+
+open Lean Qq Mathlib.Tactic
+
+class Denote {u : Level} (α : outParam (Q(Type $u))) (ε : Type) where
+  denote : ε → Q($α)
+
+export Denote (denote)
+
+class Reify {u : Level} (α : outParam Q(Type $u)) (ε : Type) (m : Type → Type) where
+  reify : Q($α) → m ε
+
+export Reify (reify)
+
+structure AtomExpr {u : Level} (α : Q(Type $u)) where
+  id   : Nat
+  expr : Q($α)
+deriving Inhabited
+
+instance {u : Level} (α : Q(Type $u)) : BEq (AtomExpr α) where
+  beq a b := a.id == b.id
+
+instance {u : Level} (α : Q(Type $u)) : Hashable (AtomExpr α) where
+  hash a := hash a.id
+
+instance {u : Level} (α : Q(Type $u)) : Reify α (AtomExpr α) AtomM where
+  reify e := (fun (id, expr) => { id, expr }) <$> AtomM.addAtom e
+
+instance {u : Level} (α : Q(Type $u)) : Denote α (AtomExpr α) where
+  denote a := a.expr
+
+
+class DenoteEq {u : Level} (α : outParam Q(Type $u)) (ε : Type) extends Denote α ε where
+  denoteEq! : ∀ e₁ e₂ : ε, Q($(denote e₁) = $(denote e₂))
+  -- denoteEq? : ∀ e₁ e₂ : ε, Option Q($(denote e₁) = $(denote e₂)) := fun e₁ e₂ => some (denoteEq! e₁ e₂)
+
+export DenoteEq (denoteEq!)
+
+-- instance (priority := low) {u : Level} (α : Q(Type $u)) (ε : Type) [Denote α ε] [BEq ε] : DenoteEq α ε where
+--   denoteEq! e₁ _ := (q(@rfl $α $(denote e₁)):)
+--   -- denoteEq? e₁ e₂ := if e₁ == e₂ then
+--   --   some (denoteEq! (α := α) e₁ e₂)
+--   -- else
+--   --   none
+
+def _root_.Qq.mkExpectedTypeHint {α : Expr} (e : Expr) : MetaM (Quoted α) :=
+  Meta.mkExpectedTypeHint e α
+
+
+
+-- open Lean Qq
+
+-- class EqClass (α : Type) (ε : outParam (α → α → Type)) where
+--   refl  : ∀ a : α, ε a a
+--   symm  : ∀ {a b : α}, ε a b → ε b a
+--   trans : ∀ {a b c : α}, ε a b → ε b c → ε a c
+
+-- export EqClass (refl symm trans)
+
+-- /-- In a `DecidableEqClass α ε`, one can check whether two expressions are equal. -/
+-- class DecidableEqClass (α : Type) (ε : outParam (α → α → Type)) extends EqClass α ε where
+--   decideEq : ∀ a b : α, Option (ε a b)
+
+-- export DecidableEqClass (decideEq)
+
+-- class NormalingEqClass (α : Type) (ε : outParam (α → α → Type)) extends EqClass α ε where
+--   normalize         : α → α
+--   normalize_eq      : ∀ a : α, ε a (normalize a)
+--   normalize_eq_symm : ∀ a : α, ε (normalize a) a := fun a => symm (normalize_eq a)
+
+-- export NormalingEqClass (normalize normalize_eq normalize_eq_symm)
+
+-- instance {α} {ε} [BEq α] [LawfulBEq α] [NormalingEqClass α ε] : DecidableEqClass α ε where
+--   decideEq a b :=
+--     if h : normalize a == normalize b then
+--       have h' := eq_of_beq h
+--       some (trans (normalize_eq a) (h' ▸ normalize_eq_symm b))
+--     else
+--       none
+
+-- /- Unfortunately, this instance cannot be nicely extended to an instance of `NormalizingEqClass` and `DecidableEqClass`,
+-- because `isDefEq` and `reduce`/`simp` require the `MetaM` monad. -/
+-- instance {u : Level} {α : Q(Sort u)} : EqClass Q($α) (fun a b => Q($a = $b)) where
+--   refl _ := q(rfl)
+--   symm h := q(($h).symm)
+--   trans h₁ h₂ := q($(h₁).trans $h₂)
+
+-- instance {u : Level} {α : Q(Sort u)} : DecidableEqClass Q($α) (fun a b => Q($a = $b)) where
+--   decideEq a b :=
+--     if a.equal b then
+--       some (refl a:)
+--     else
+--       none
+
+
+
+-- /--
+-- An `ExprEqClass α ε` is a type that can represent expressions (in `α`)
+-- and reason about their equality (in `ε`).
+-- -/
+-- class ExprEqClass (α : Type) (ε : outParam (α → α → Type)) extends EqClass α ε where
+--   u : Level
+--   αExpr : Q(Type $u)
+--   denote : α → Q($αExpr)
+--   toProofExpr : ∀ a b : α, (eq : ε a b) → Q($(toExpr a) = $(toExpr b))
+
+-- -- /--
+-- -- An `Abstraction α β` represents that expressions in `α` can be used to reason about
+-- -- expressions in `β`.
+-- -- -/
+-- -- class Abstraction (α : Type → Type)  where
+-- --   abstract : ∀ β, β → α β
+-- --   original : ∀ β, α β → β
+-- -- #check Pure
