HumanProof/Meta/Lemmas.lean
@@ -1,0 +1,32 @@
+
+universe u
+
+variable {α : Type u}
+
+theorem _root_.List.merge_ne_nil_of_right {le} {xs ys : List α} (hy : ys ≠ []) : xs.merge ys le ≠ [] := by
+  cases xs with
+  | nil => simp [hy]
+  | cons =>
+    cases ys with
+    | nil => contradiction
+    | cons => unfold List.merge; split <;> simp
+
+theorem _root_.List.merge_ne_nil_of_left {le} {xs ys : List α} (hx : xs ≠ []) : xs.merge ys le ≠ [] := by
+  cases xs with
+  | nil => contradiction
+  | cons =>
+    cases ys with
+    | nil => simp
+    | cons => unfold List.merge; split <;> simp
+
+@[simp]
+theorem _root_.List.count_merge [BEq α] {le : α → α → Bool} (l₁ l₂ : List α) (a : α) :
+    (l₁.merge l₂ le).count a = l₁.count a + l₂.count a := by
+  induction l₁ generalizing l₂ with
+  | nil => simp
+  | cons x l₁ ih₁ =>
+    induction l₂ with
+    | nil => simp
+    | cons y l₂ ih₂ =>
+      unfold List.merge
+      split <;> simp only [List.count_cons, ih₁, ih₂] <;> split <;> omega
